examples/scache/ArrayPtr.s.dfy
@@ -1,0 +1,66 @@
+module Ptrs {
+  type {:extern} PtrInternalOpaqueType(!new,==)
+
+  // Non-ghosty
+
+  datatype Ptr = Ptr(_internal: PtrInternalOpaqueType)
+
+  function method nullptr() : Ptr
+
+  // Ghosty
+
+  // TODO there needs to be some way to enforce that the
+  // impl cannot conjure these out of nowhere
+
+  datatype R<V> =
+    | ArrayReadCount(ptr: Ptr, s: seq<V>, refcount: int)
+    | ConstArrayDeref(ptr: Ptr, s: seq<V>)
+
+  type ArrayDeref<V> = r: R<V> | r.ArrayReadCount? && r.refcount == 0
+      witness ArrayReadCount(nullptr(), [], 0)
+
+  type ConstArrayDeref<V> = r: R<V> | r.ConstArrayDeref?
+      witness ConstArrayDeref(nullptr(), [])
+
+  method {:extern} array_write<V>(p: Ptr, linear inout d: ArrayDeref, i: int, v: V)
+  requires old_d.ptr == p
+  requires 0 <= i < |old_d.s|
+  ensures d == d.(s := old_d.s[i := v])
+
+  method {:extern} array_read<V>(p: Ptr, shared d: ArrayDeref<V>, i: int)
+  returns (v: V)
+  requires d.ptr == p
+  requires 0 <= i < |d.s|
+  ensures v == d.s[i]
+
+  method {:extern} const_array_read<V>(p: Ptr, shared d: ConstArrayDeref<V>, i: int)
+  returns (v: V)
+  requires d.ptr == p
+  requires 0 <= i < |d.s|
+  ensures v == d.s[i]
+
+  predicate transform<V(!new)>(a: multiset<R<V>>, b: multiset<R<V>>)
+  {
+    || (exists ptr, s, refcount ::
+      && a == multiset{ArrayReadCount(ptr, s, refcount)}
+      && b == multiset{ArrayReadCount(ptr, s, refcount + 1), ConstArrayDeref(ptr, s)}
+    )
+    || (exists ptr, s, refcount, s' ::
+      && a == multiset{ArrayReadCount(ptr, s, refcount), ConstArrayDeref(ptr, s')}
+      && b == multiset{ArrayReadCount(ptr, s, refcount - 1)}
+    ) 
+  }
+
+  /*method main(p: Ptr, linear d: ArrayDeref<int>)
+  returns (linear d': ArrayDeref<int>)
+  requires |d.s| == 1
+  requires d.ptr == p
+  {
+    var a := array_read(p, d, 0);
+    d' := d;
+  }*/
+
+  // forall C, D . rel(C, D) ==> exists C', D' . (A+C) ==> (A'+C') & (B+D) ==> (B'+D') & rel(C',D')
+  // ------
+  // A+B ==> A'+B'
+}
