examples/scache/AtomicStatus.i.dfy
@@ -1,0 +1,156 @@
+include "Atomic.s.dfy"
+include "RWLock.i.dfy"
+include "ArrayPtr.s.dfy"
+include "../../lib/Lang/NativeTypes.s.dfy"
+include "../../lib/Lang/LinearMaybe.s.dfy"
+
+module AtomicStatusImpl {
+  import opened NativeTypes
+  import opened Ptrs
+  import opened AtomicSpec
+  import opened LinearMaybe
+  import ReadWriteLockResources
+
+  const flag_free : uint8 := 0;
+  const flag_back : uint8 := 1;
+  const flag_write : uint8 := 2;
+  const flag_back_write : uint8 := 3;
+
+  type AtomicStatus = Atomic<uint8, ReadWriteLockResources.R>
+
+  predicate state_inv(v: uint8, g: ReadWriteLockResources.R, ptr: Ptr)
+  {
+    && g.FlagsField?
+    && g.ptr == ptr
+    && (g.flags == ReadWriteLockResources.Free ==> v == flag_free)
+    && (g.flags == ReadWriteLockResources.Back ==> v == flag_back)
+    && (g.flags == ReadWriteLockResources.Write ==> v == flag_write)
+    && (g.flags == ReadWriteLockResources.Back_PendingWrite ==>
+        v == flag_back_write)
+  }
+
+  predicate atomic_status_inv(a: AtomicStatus, ptr: Ptr)
+  {
+    forall v, g :: atomic_inv(a, v, g) <==> state_inv(v, g, ptr)
+  }
+
+  method unsafe_obtain<R>() returns (linear r: R)
+  method unsafe_dispose<R>(linear r: R)
+
+  method try_acquire_writeback(a: AtomicStatus, ptr: Ptr)
+  returns (success: bool, linear m: maybe<ReadWriteLockResources.R>)
+  requires atomic_status_inv(a, ptr)
+  ensures !success ==> !has(m)
+  ensures success ==> has(m)
+      && read(m) == ReadWriteLockResources.BackObtained(ptr)
+  {
+    var did_set := compare_and_set(a, flag_free, flag_back);
+
+    ///// Begin jank
+    ///// Setup:
+    var v1 := flag_free;
+    var v2 := flag_back;
+    var old_v: uint8;
+    var new_v: uint8;
+    linear var old_g: ReadWriteLockResources.R := unsafe_obtain();
+    assume old_v == v1 ==> new_v == v2 && did_set;
+    assume old_v != v1 ==> new_v == old_v && !did_set;
+    assume atomic_inv(a, old_v, old_g);
+    linear var new_g;
+    ///// Transfer:
+    if did_set {
+      linear var res;
+      new_g, res := ReadWriteLockResources.transform_TakeBack(ptr, old_g);
+      m := give(res);
+    } else {
+      m := empty();
+      new_g := old_g;
+    }
+    assert state_inv(new_v, new_g, ptr);
+    ///// Teardown:
+    assert atomic_inv(a, new_v, new_g);
+    unsafe_dispose(new_g);
+    ///// End jank
+
+    success := did_set;
+  }
+
+  method try_set_write_lock(a: AtomicStatus, ptr: Ptr)
+  returns (success: bool, linear m: maybe<ReadWriteLockResources.R>)
+  requires atomic_status_inv(a, ptr)
+  ensures !success ==> !has(m)
+  ensures success ==> has(m)
+      && read(m) == ReadWriteLockResources.WritePendingAwaitBack(ptr)
+  {
+    var orig_value := fetch_or(a, flag_write);
+
+    ///// Begin jank
+    ///// Setup:
+    var v := flag_write;
+    var old_v: uint8;
+    var new_v: uint8;
+    linear var old_g: ReadWriteLockResources.R := unsafe_obtain();
+    assume orig_value == old_v;
+    assume new_v == bit_or(old_v, v);
+    assume atomic_inv(a, old_v, old_g);
+    linear var new_g;
+    ///// Transfer:
+    var fl := old_g.flags;
+    if fl == ReadWriteLockResources.Free {
+      linear var r;
+      new_g, r := ReadWriteLockResources.transform_TakeWrite(ptr, old_g);
+      m := give(r);
+    } else if fl == ReadWriteLockResources.Back {
+      linear var r;
+      new_g, r := ReadWriteLockResources.transform_TakeWriteAwaitBack(ptr, old_g);
+      m := give(r);
+    } else {
+      new_g := old_g;
+      m := empty();
+    }
+    ///// Teardown:
+    assert atomic_inv(a, new_v, new_g);
+    unsafe_dispose(new_g);
+    ///// End jank
+
+    success := bit_and(orig_value, flag_write) == 0;
+  }
+
+  method try_check_writeback_isnt_set(a: AtomicStatus, ptr: Ptr,
+      linear m: ReadWriteLockResources.R)
+  returns (success: bool, linear m': ReadWriteLockResources.R)
+  requires atomic_status_inv(a, ptr)
+  requires m == ReadWriteLockResources.WritePendingAwaitBack(ptr)
+  ensures !success ==> m' == m
+  ensures success ==> m' == ReadWriteLockResources.WritePending(ptr, 0)
+  {
+    var f := atomic_read(a);
+
+    ///// Begin jank
+    ///// Setup:
+    var v := flag_write;
+    var old_v: uint8;
+    var new_v: uint8;
+    linear var old_g: ReadWriteLockResources.R := unsafe_obtain();
+    assume new_v == old_v;
+    assume f == old_v;
+    assume atomic_inv(a, old_v, old_g);
+    linear var new_g;
+    ///// Transfer:
+    var fl := old_g.flags;
+    if fl == ReadWriteLockResources.Free
+        || fl == ReadWriteLockResources.Write
+    {
+      new_g, m' := ReadWriteLockResources.transform_TakeWriteFinishBack(ptr, fl, old_g, m);
+    } else {
+      new_g := old_g;
+      m' := m;
+    }
+    ///// Teardown:
+    assert atomic_inv(a, new_v, new_g);
+    unsafe_dispose(new_g);
+    ///// End jank
+
+    success := bit_and(f, flag_back) == 0;
+  }
+}
