examples/scache/Cache.i.dfy
@@ -1,0 +1,7 @@
+module CacheImpl {
+  datatype Cache = Cache(
+    data: seq<Ptr>,
+    status: seq<AtomicStatus>,
+    read_locks: seq<seq<AtomicRefcount>
+  )
+}
