examples/scache/RWLock.i.dfy
@@ -1,0 +1,165 @@
+include "ArrayPtr.s.dfy"
+
+module ReadWriteLockResources {
+  import Ptrs
+
+  function NThreads() : int { 24 }
+
+  /*
+   * We consider two bits of the status field, WriteLock and WriteBack.
+   * To avoid confusion, I simply call them 'Write' and 'Back'.
+   *
+   * Write and Back. Of course, 'Write'
+   * and 'Back' should be exclusive operations;
+   * When both flags are set,
+   * it should be interpreted as the 'Write' being
+   * pending, with the 'Back' being in progress.
+   */
+  datatype Flag =
+    | Free
+    | Back
+    | Write
+    | Back_PendingWrite
+
+  datatype R =
+    | FlagsField(ptr: Ptrs.Ptr, flags: Flag)
+    | ReadRefCount(ptr: Ptrs.Ptr, t: int, refcount: int)
+
+    | ReadPending(ptr: Ptrs.Ptr, t: int)
+    | ReadObtained(ptr: Ptrs.Ptr, t: int)
+    
+    | BackObtained(ptr: Ptrs.Ptr)
+
+    | WritePendingAwaitBack(ptr: Ptrs.Ptr)
+    | WritePending(ptr: Ptrs.Ptr, visited: int)
+    | WriteObtained(ptr: Ptrs.Ptr)
+
+  datatype Step =
+    | TakeBackStep(ptr: Ptrs.Ptr)
+    | TakeWrite(ptr: Ptrs.Ptr)
+    | TakeWriteAwaitBack(ptr: Ptrs.Ptr)
+
+  predicate TakeBack(a: multiset<R>, b: multiset<R>, ptr: Ptrs.Ptr)
+  {
+    && a == multiset{ FlagsField(ptr, Free) }
+    && b == multiset{
+      FlagsField(ptr, Back),
+      BackObtained(ptr)
+    }
+  }
+
+  predicate TakeWrite(a: multiset<R>, b: multiset<R>, ptr: Ptrs.Ptr)
+  {
+    && a == multiset{ FlagsField(ptr, Free) }
+    && b == multiset{
+      FlagsField(ptr, Write),
+      WritePendingAwaitBack(ptr)
+    }
+  }
+
+  predicate TakeWriteAwaitBack(a: multiset<R>, b: multiset<R>, ptr: Ptrs.Ptr)
+  {
+    && a == multiset{ FlagsField(ptr, Back) }
+    && b == multiset{
+      FlagsField(ptr, Back_PendingWrite),
+      WritePendingAwaitBack(ptr)
+    }
+  }
+
+  predicate TakeWriteFinishBack(a: multiset<R>, b: multiset<R>, ptr: Ptrs.Ptr, fl: Flag)
+  {
+    // The 'free' case cannot actually occur, but it's convenient to allow it.
+    && (fl == Write || fl == Free)
+    && a == multiset{
+      FlagsField(ptr, fl),
+      WritePendingAwaitBack(ptr)
+    }
+    && b == multiset{
+      FlagsField(ptr, fl),
+      WritePending(ptr, 0)
+    }
+  }
+
+  predicate TakeWriteCheckReadZero(a: multiset<R>, b: multiset<R>, ptr: Ptrs.Ptr, idx: int)
+  {
+    && a == multiset{
+      WritePending(ptr, idx),
+      ReadRefCount(ptr, idx, 0) 
+    }
+    && b == multiset{
+      WritePending(ptr, idx + 1),
+      ReadRefCount(ptr, idx, 0) 
+    }
+  }
+
+  predicate TakeWriteFinish(a: multiset<R>, b: multiset<R>, ptr: Ptrs.Ptr)
+  {
+    && a == multiset{
+      WritePending(ptr, NThreads())
+    }
+    && b == multiset{
+      WriteObtained(ptr)
+    }
+  }
+
+  predicate TakeRead(a: multiset<R>, b: multiset<R>, ptr: Ptrs.Ptr, t: int, r: int)
+  {
+    && a == multiset{
+      ReadRefCount(ptr, t, r)
+    }
+    && a == multiset{
+      ReadRefCount(ptr, t, r+1),
+      ReadPending(ptr, t)
+    }
+  }
+
+  predicate TakeReadFinish(a: multiset<R>, b: multiset<R>, ptr: Ptrs.Ptr, t: int, r: int, fl: Flag)
+  {
+    && (fl == Free || fl == Back)
+    && a == multiset{
+      ReadPending(ptr, t),
+      FlagsField(ptr, fl)
+    }
+    && a == multiset{
+      ReadObtained(ptr, t)
+    }
+  }
+
+  predicate TakeReadBail(a: multiset<R>, b: multiset<R>, ptr: Ptrs.Ptr, t: int, r: int)
+  {
+    && a == multiset{
+      ReadRefCount(ptr, t, r),
+      ReadPending(ptr, t)
+    }
+    && b == multiset{
+      ReadRefCount(ptr, t, r-1)
+    }
+  }
+
+  method transform_TakeBack(ptr: Ptrs.Ptr, linear s: R)
+  returns (linear t: R, linear u: R)
+  requires s == FlagsField(ptr, Free)
+  ensures t == FlagsField(ptr, Back)
+  ensures u == BackObtained(ptr)
+
+  method transform_TakeWrite(ptr: Ptrs.Ptr, linear s: R)
+  returns (linear t: R, linear u: R)
+  requires s == FlagsField(ptr, Free)
+  ensures t == FlagsField(ptr, Write)
+  ensures u == WritePendingAwaitBack(ptr)
+
+  method transform_TakeWriteAwaitBack(ptr: Ptrs.Ptr, linear s: R)
+  returns (linear t: R, linear u: R)
+  requires s == FlagsField(ptr, Back)
+  ensures t == FlagsField(ptr, Back_PendingWrite)
+  ensures u == WritePendingAwaitBack(ptr)
+
+
+  method transform_TakeWriteFinishBack(ptr: Ptrs.Ptr, fl: Flag, linear s1: R, linear s2: R)
+  returns (linear t1: R, linear t2: R)
+  requires fl == Write || fl == Free
+  requires s1 == FlagsField(ptr, fl)
+  requires s2 == WritePendingAwaitBack(ptr)
+  ensures t1 == FlagsField(ptr, fl)
+  ensures t2 == WritePending(ptr, 0)
+}
